Predeclare Lean Nat decidable equality

src/lean.ml
@@ -932,6 +932,8 @@ type core_shape = Legacy | Modern
 
 type predeclared_ind_kind =
   | Eq
+  | False
+  | Decidable
   | Bool
   | Nat
   | Nat_le
@@ -951,12 +953,15 @@ type predeclared_def_kind =
   | Beq
   | Ble
   | Blt
+  | Nat_decEq
   | Nat_isValidChar
 type predeclared_ind_as_def_kind = ULift_cumul
 
 let get_predeclared_cnames (k : predeclared_ind_kind) n =
   match k with
   | Eq -> [ N.append n "refl" ]
+  | False -> []
+  | Decidable -> [ N.append n "isFalse"; N.append n "isTrue" ]
   | Bool -> [ N.append n "false"; N.append n "true" ]
   | Nat -> [ N.append n "zero"; N.append n "succ" ]
   | Nat_le -> [ N.append n "refl"; N.append n "step" ]
@@ -985,6 +990,8 @@ let get_predeclared_ind_any ~ctors ~uint32_is_legacy n i =
       |> Option.map (fun x -> (indk, indh, x)))
     [
       (Eq, [ "Eq" ]);
+      (False, [ "False" ]);
+      (Decidable, [ "Decidable" ]);
       (Bool, [ "Bool" ]);
       (Nat, [ "Nat" ]);
       (Nat_le, [ "Nat"; "le" ]);
@@ -1034,6 +1041,7 @@ let get_predeclared_def_any n i =
       (Beq, [ "Nat"; "beq" ]);
       (Ble, [ "Nat"; "ble" ]);
       (Blt, [ "Nat"; "blt" ]);
+      (Nat_decEq, [ "Nat"; "decEq" ]);
       (Nat_isValidChar, [ "Nat"; "isValidChar" ]);
     ]
 
@@ -3402,6 +3410,7 @@ and declare_def { name = n; ty; body; univs; } i =
           | Beq
           | Ble
           | Blt
+          | Nat_decEq
           | Nat_isValidChar ),
           _,
           (def_name, c) ) ->
@@ -3569,7 +3578,9 @@ and declare_ind { name = n; params; ty; ctors; univs } i =
         squashy,
         [] )
     | Some
-        ( ( ( Bool
+        ( ( ( False
+            | Decidable
+            | Bool
             | Nat
             | Nat_le
             | Or
